

SUBJECT: ENGINEERING MATHEMATICS-I [MAT 1151] (CHEMISTRY CYCLE)
SCHEME OF EVALUATION

Q. No.	DESCRIPTION	MARKS
1A Solution	<p>Solve $y - \cos x \frac{dy}{dx} = y^2 (1 - \sin x) \cos x$ given $y(0) = 2$.</p> <p>To solve: $-\cos x \frac{dy}{dx} = y^2 (1 - \sin x) \cos x - y$</p> <p>Divide by $y^2 \cos x$,</p> <p>Then, $\frac{-1}{y^2} \frac{dy}{dx} + \frac{1}{y} \sec x = 1 - \sin x$</p> <p>Substitute $\frac{1}{y} = z$, then $\frac{-1}{y^2} \frac{dy}{dx} = \frac{dz}{dx}$</p> <p>The above DE, $\frac{dz}{dx} + z \sec x = 1 - \sin x$ which is linear in z.</p> <p>I.F = $e^{\int \sec x dx} = e^{\log(\sec x + \tan x)} = \sec x + \tan x$</p> <p>The general solution in z is,</p> $z(\sec x + \tan x) = \int (1 - \sin x)(\sec x + \tan x) dx$ <p>By back substituting y, $\frac{(\sec x + \tan x)}{y} = \int (1 - \sin x) \frac{(1 + \sin x)}{\cos x} dx + c$</p> <p>By simplifying, $\frac{(\sec x + \tan x)}{y} = \int \cos x dx + c$</p> <p>i.e., $\frac{(\sec x + \tan x)}{y} = \sin x + c$</p> <p>By substituting the initial condition, $y(0) = 2$, the value of $c = 0.5$.</p> <p>The particular solution is, $\sec x + \tan x = y \sin x + \frac{y}{2}$</p>	<p align="center">1</p> <p align="center">1</p> <p align="center">1</p> <p align="center">1</p>
1B Solution	<p>Solve $(2x - 1)^3 y''' + (2x - 1)y' - 2y = 8x^2 - 2x + 3$.</p> <p>By substituting, $(2x - 1) = e^t$. Then, $x = \frac{e^t + 1}{2}$ and $t = \log(2x - 1)$.</p> <p>The above DE, $(2^3 D(D - 1)(D - 2) + 2D - 2)y = 2e^{2t} + 3e^t + 4$</p> <p>A.E, $8m^3 - 24m^2 + 18m - 2 = 0$</p> <p>Roots are $1, \left(1 \pm \frac{\sqrt{3}}{2}\right)$</p> <p>The complementary function is, $y_c = c_1 e^t + c_2 e^{(1 + \frac{\sqrt{3}}{2})t} + c_3 e^{(1 - \frac{\sqrt{3}}{2})t}$</p> <p>The particular integral, $y_p = \frac{1}{8D^3 - 24D^2 + 18D - 2} (2e^{2t} + 3e^t + 4)$</p> <p>i.e, $y_p = \frac{2e^{2t}}{2} + \frac{3te^t}{18} - \frac{4}{2}$</p> <p>Therefore, $y = c_1(2x - 1) + c_2(2x - 1)^{(1 + \frac{\sqrt{3}}{2})} + c_3(2x - 1)^{(1 - \frac{\sqrt{3}}{2})} + (2x - 1)^2 + \frac{(2x - 1)\log(2x - 1)}{6} - 2$.</p>	<p align="center">1.5</p> <p align="center">0.5</p> <p align="center">1</p> <p align="center">0.5</p> <p align="center">1.5</p> <p align="center">1</p>

2A	<p>Using Lagrange's interpolation formula find $y(7)$ from the following table.</p> <table><tr><td>x</td><td>5</td><td>6</td><td>9</td><td>11</td></tr><tr><td>y</td><td>12</td><td>13</td><td>14</td><td>16</td></tr></table>	x	5	6	9	11	y	12	13	14	16	
x	5	6	9	11								
y	12	13	14	16								
Solution	<p>We have, By Lagrange's interpolation formula, $x = 7, x_0 = 5, x_1 = 6, x_2 = 9, x_3 = 11, y_0 = 12, y_1 = 13, y_2 = 14, y_3 = 16.$</p> <p>From the formula, $y = f(x) = \frac{(x-x_1)(x-x_2)(x-x_3)}{(x_0-x_1)(x_0-x_2)(x_0-x_3)}y_0 + \frac{(x-x_0)(x-x_2)(x-x_3)}{(x_1-x_0)(x_1-x_2)(x_1-x_3)}y_1 + \frac{(x-x_0)(x-x_1)(x-x_3)}{(x_2-x_0)(x_2-x_1)(x_2-x_3)}y_2 + \frac{(x-x_0)(x-x_1)(x-x_2)}{(x_3-x_0)(x_3-x_1)(x_3-x_2)}y_3$</p> $= \frac{(7-6)(7-9)(7-11)}{(5-6)(5-9)(5-11)}(12) + \frac{(7-5)(7-9)(7-11)}{(6-5)(6-9)(6-11)}(13)$ $+ \frac{(7-5)(7-6)(7-11)}{(9-5)(9-6)(9-11)}(14)$ $+ \frac{(7-5)(7-6)(7-9)}{(11-5)(11-6)(11-9)}(16)$ $= -\frac{96}{24} + \frac{208}{15} + \frac{112}{24} - \frac{64}{60} = 13.4667$	<p>1</p> <p>3</p>										
2B	<p>Solve the initial value problem, $\frac{dy}{dx} = \frac{y^2-x^2}{y^2+x^2}, y(0) = 1$ at $x = 0.2$ by using Modified Euler's method, take $h = 0.1$. Modify the solution twice in each step. Use this value $y(0.2)$ and find y at $x = 0.3$ using Runge - Kutta method of order 4 with $h = 0.1$.</p>											
Solution	<p>To find $y(0.2)$ using Modified Euler's method, $h = 0.1$ $x_0 = 0, x_1 = 0.1, x_2 = 0.2$</p> $y_1^{(0)} = 1.1$ $y_1^{(1)} = 1.0991535$ $y_1^{(2)} = 1.099179$ <p>Thus, $y(0.1) = 1.099179$</p> $y_2^{(0)} = 1.197537$ $y_2^{(1)} = 1.1950115$ $y_2^{(2)} = 1.1956333$ <p>Thus, $y(0.2) = 1.1956333$</p> <p>R-K method to find $y(0.3)$:</p> $k_1 = 0.094556,$ $k_2 = 0.092227,$ $k_3 = 0.09221,$ $k_4 = 0.08971,$ <p>Hence, $y(0.3) = 1.28779$</p>	<p>1.5</p> <p>1.5</p> <p>0.5</p> <p>0.5</p> <p>0.5</p> <p>0.5</p> <p>1</p>										

<div>3A</div> <div>Solution</div>	<div> <div>The following table gives the velocity of a particle at time t.</div> <table border="1"> <tr> <th>t(sec)</th><th>0</th><th>2</th><th>4</th><th>6</th><th>8</th><th>10</th><th>12</th></tr> <tr> <th>v (m/sec)</th><td>4</td><td>6</td><td>16</td><td>34</td><td>60</td><td>94</td><td>136</td></tr> </table> <div>Find the distance moved by the particle in 12 sec and the acceleration at t = 2 sec.</div> <div>We know $\frac{ds}{dt} = v, \frac{dv}{dt} = a$</div> <div>Where v = velocity; a = acceleration and s = distance</div> <div>$\therefore ds = v dt \Rightarrow s = \int v dt$</div> <div>$\therefore$ The distance moved by the particle in 12 sec = $\int_0^{12} v dt$.</div> <div>Here h = 2. By Simpson's $\frac{1}{3}$ rule,</div> <div>$\therefore \int_0^{12} v dt = \frac{h}{3} [(v_0 + v_6) + 4(v_1 + v_3 + v_5) + 2(v_2 + v_4)]$</div> <div>$= \frac{2}{3} [(4 + 136) + 4(6 + 34 + 94) + 2(16 + 60)] = 552$</div> <div>$\therefore$ Distance covered = 552 meters</div> <div>$Acceleration = \left(\frac{dv}{dt}\right)_{t=2}$</div> <table> <tr> <th>t</th><th>v</th><th>Δv</th><th>$\Delta^2 v$</th></tr> <tr><td>0</td><td>4</td><td></td><td></td></tr> <tr><td></td><td></td><td>2</td><td></td></tr> <tr><td>2</td><td>6</td><td></td><td>8</td></tr> <tr><td></td><td></td><td>10</td><td></td></tr> <tr><td>4</td><td>16</td><td></td><td>8</td></tr> <tr><td></td><td></td><td>18</td><td></td></tr> <tr><td>6</td><td>34</td><td></td><td>8</td></tr> <tr><td></td><td></td><td>26</td><td></td></tr> <tr><td>8</td><td>60</td><td></td><td>8</td></tr> <tr><td></td><td></td><td>34</td><td></td></tr> <tr><td>10</td><td>94</td><td></td><td>8</td></tr> <tr><td></td><td></td><td>42</td><td></td></tr> <tr><td>12</td><td>136</td><td></td><td></td></tr> </table> <div>Thus, acceleration is, $\left(\frac{dv}{dt}\right)_t = \frac{1}{h} \left(\Delta y_0 - \frac{\Delta^2 y_0}{2} + \dots\right)$</div> <div>$= \frac{1}{2} \left(10 - \frac{8}{2}\right) = 3m/sec^2$</div> </div>	t(sec)	0	2	4	6	8	10	12	v (m/sec)	4	6	16	34	60	94	136	t	v	Δv	$\Delta^2 v$	0	4					2		2	6		8			10		4	16		8			18		6	34		8			26		8	60		8			34		10	94		8			42		12	136		
		t(sec)	0	2	4	6	8	10	12																																																																
		v (m/sec)	4	6	16	34	60	94	136																																																																
		t	v	Δv	$\Delta^2 v$																																																																				
		0	4																																																																						
				2																																																																					
		2	6		8																																																																				
				10																																																																					
		4	16		8																																																																				
				18																																																																					
6	34		8																																																																						
		26																																																																							
8	60		8																																																																						
		34																																																																							
10	94		8																																																																						
		42																																																																							
12	136																																																																								
1																																																																									
2																																																																									
1																																																																									

3B	<p>Solve the system of equations, correct to 4 decimal places by using Gauss - Seidel method:</p> <p>$x + 4y + 2z = 15$; $5x + 2y + z = 12$; $x + 2y + 5z = 20$, Carryout 3 iterations.</p>																					
Solution	<p>Re-write the system of equations in Diagonally dominant form</p> $x = \frac{12-2y-z}{5}; \quad y = \frac{15-x-2z}{4}; \quad z = \frac{20-x-2y}{5}$ <table><tr><td>Iteration</td><td>x</td><td>y</td><td>z</td></tr><tr><td>0</td><td>0</td><td>0</td><td>0</td></tr><tr><td>1</td><td>2.4</td><td>3.15</td><td>2.26</td></tr><tr><td>2</td><td>0.688</td><td>2.448</td><td>2.8832</td></tr><tr><td>3</td><td>0.8442</td><td>2.0974</td><td>2.9922</td></tr></table>	Iteration	x	y	z	0	0	0	0	1	2.4	3.15	2.26	2	0.688	2.448	2.8832	3	0.8442	2.0974	2.9922	<p>0.5</p> <p>0.5M for each iteration</p>
Iteration	x	y	z																			
0	0	0	0																			
1	2.4	3.15	2.26																			
2	0.688	2.448	2.8832																			
3	0.8442	2.0974	2.9922																			
3C	<p>Find all the eigenvalues and an eigenvector corresponding to the least eigenvalue of the matrix</p> $A = \begin{bmatrix} 6 & -2 & -2 \\ -2 & 6 & -1 \\ -1 & -1 & 5 \end{bmatrix}$																					
Solution	<p>The characteristic equation of matrix A is $\det(A - \lambda I) = 0$</p> $\lambda^3 - 17\lambda^2 + 90\lambda - 144 = 0$ <p>The eigenvalues are $\lambda = 3, 8, 6$</p> <p>The eigenvector corresponding to $\lambda = 3$ is $[A - 3I]X = 0$</p> $\begin{bmatrix} 3 & -2 & -1 \\ -2 & 3 & -1 \\ -1 & -1 & 2 \end{bmatrix} \begin{bmatrix} x \\ y \\ z \end{bmatrix} = \begin{bmatrix} 0 \\ 0 \\ 0 \end{bmatrix}$ $\frac{x}{5} = \frac{-y}{-5} = \frac{z}{5} = k$ <p>Thus $X = [k, k, k]^T, k \in R$ is the eigenvector.</p>	<p>1.5</p> <p>1</p> <p>1</p> <p>0.5</p>																				

4A	Find a multiple root of the equation using Newton's method, $x^3 - x^2 - 8x + 12 = 0$. Take $x_0 = 1.8$.	
Solution	<p>Newton's method for multiple roots, with $x_0 = 1.8$</p> $x_0 - 3 \frac{f(x_0)}{f'(x_0)} = 2.10638$ $x_0 - 2 \frac{f'(x_0)}{f''(x_0)} = 2.22727$ $x_0 - \frac{f''(x_0)}{f'''(x_0)} = 0.33333$ <p>Double root at 2. Let us take $x_1 = 2.10638$</p> $x_0 - 2 \frac{f(x_0)}{f'(x_0)} = 2.0011$ $x_0 - \frac{f'(x_0)}{f''(x_0)} = 2.00319$ <p>The approximate root correct to 2 decimal places is 2.</p>	<p>2</p> <p>2</p>
4B	Express the vector $(1, -2, 5)$ as a linear combination of the vectors $\{(1, 1, 1), (1, 2, 3), (2, -1, 1)\}$ in \mathbb{R}^3.	
Solution	<p>Let $(1, -2, 5) = a(1, 1, 1) + b(1, 2, 3) + c(2, -1, 1)$</p> $= (a + b + 2c, a + 2b - c, a + 3b + c)$ <p>Equating and solving: $a = -6, b = 3, c = 2$.</p>	<p>1</p> <p>1</p>
4C	Construct an orthonormal basis using Gram-Schmidt orthogonalization process from the set of linearly independent vectors $\{v_1 = (1, 0, 1), v_2 = (1, 0, -1), v_3 = (0, 3, 4)\}$.	
Solution	$u_1 = \frac{v_1}{\ v_1\ } = \frac{(1, 0, 1)}{\sqrt{1^2 + 0^2 + 1^2}} = \left(\frac{1}{\sqrt{2}}, 0, \frac{1}{\sqrt{2}}\right)$ <p>Now $a_2 = v_2 - (v_2 \cdot u_1)u_1 = (1, 0, -1) - 0 \cdot \left(\frac{1}{\sqrt{2}}, 0, \frac{1}{\sqrt{2}}\right) = (1, 0, -1)$</p> <p>and $u_2 = \frac{a_2}{\ a_2\ } = \frac{(1, 0, -1)}{\sqrt{1^2 + 0^2 + (-1)^2}} = \left(\frac{1}{\sqrt{2}}, 0, -\frac{1}{\sqrt{2}}\right)$</p> $a_3 = v_3 - (v_3 \cdot u_2)u_2 - (v_3 \cdot u_1)u_1 = (0, 3, 0)$ $u_3 = \frac{a_3}{\ a_3\ } = \frac{(0, 3, 0)}{\sqrt{0^2 + 3^2 + 0^2}} = (0, 1, 0).$ <p>Hence the required set of orthonormal vectors is $\left(\frac{1}{\sqrt{2}}, 0, \frac{1}{\sqrt{2}}\right), \left(\frac{1}{\sqrt{2}}, 0, -\frac{1}{\sqrt{2}}\right), (0, 1, 0)$</p>	<p>1</p> <p>1</p> <p>1</p> <p>0.5</p> <p>0.5</p>